# 变量替换法

### 齐次方程



$$
f(x,y)= \frac{x^3+x^2y+y^3}{xy^2} \\ = \frac{1+\frac{y}{x}+(\frac{y}{x})^3}{(\frac{y}{x})^2} \\ 即形如 \frac{dy}{dx}=g(\frac{y}{x}),叫做齐次方程
$$



$$
令\frac{y}{x}=u \\ y=ux \\ \frac{dy}{dx}=u+x\frac{du}{dx} \\ u + x\frac{du}{dx} =g(u) \\  x\frac{du}{dx} = g(u)-u \\ 1) 当g(u) - u\neq 0 \\ \int \frac{du}{g(u)-u}=\int \frac{dx}{x}\\ G(u)=ln|x|+C \\ G(\frac{x}{y})=ln|x|+C \\ 2)当g(u_0)-u_0=0时 \\ \frac{y}{x} = u_0 \\ y=u_0x
$$

$$
例：求y'=\frac{y+\sqrt{x^2+y^2}}{x}\quad y(1)=0的特解
$$

$$
\frac{dy}{dx}=\frac{y}{x}+\sqrt{1+(\frac{y}{x})^2}
$$

$$
令\frac{y}{x}=u
$$

$$
u+x\frac{du}{dx}=u+\sqrt{1+u^2} \\ \int \frac{du}{\sqrt{1+u^2}}=\int \frac{dx}{x}
$$

$$
设u= \tan{t} \quad du=\sec^2{t} \\ \int \sec t dt=ln|\sec t + \tan t|\\ =ln|u+\sqrt{1+u^2}|
$$

$$
\therefore ln|u+\sqrt{1+u^2}|=ln|x|+lnC \\ \frac{u+\sqrt{1+u^2}}{x}=C \\ \frac{y}{x}+\frac{\sqrt{x^2+y^2}}{x}=Cx
$$

$$
\because y(1)=0 \\ \therefore C=1 \\ y+\sqrt{x^2+y^2}=x^2 \\ y=\frac{1}{2}(x^2-1)
$$

### 能化成齐次方程的方程

$$
\frac{dy}{dx}=f(\frac{a_1x+b_1y+c_1}{a_2x+b_2y+c_2})
$$

$$
1)c_1=c_2=0
$$

$$
2)c_1^2+c_2^2 \neq 0
$$

$$
(1) \frac{a_1}{a_2}=\frac{b_1}{b_2}=\frac{c_1}{c_2}=k \\ \therefore y=kx+b
$$

$$
(2) \frac{a_1}{a_2}=\frac{b_1}{b_2}\neq \frac{c_1}{c_2} \\ f(\frac{k(a_{2}x+b_2y)+c_2}{a_2x+b_2y+c_2}) \\ 令a_2x+b_2y=u \\ a_2dx+b_2dy=du \\ a_2+b_2\frac{dy}{dx}=\frac{du}{dx} \\ (\frac{du}{dx}-a_2)\frac{1}{b_2}=f(u)\\ \therefore \frac{du}{dx}=b_2f(u)+a_2
$$

$$
(3)\frac{a_1}{a_2} \neq \frac{b_1}{b_2}
$$

$$
令 \quad \begin{cases}
a_1x+b_1y+c_1=0\\
a_2x+b_2y+c_2=0\\
\end{cases} \\ 解得(x,y)=(\alpha,\beta) \\ 令\quad  x- \alpha=X \\ y- \beta =Y \\ \frac{dY}{dX} =  \frac{a_1X+b_1Y}{a_2X+b_2Y}
$$

&#x20;例 ​$$(x-y-1)dx+(4y+x-1dy)=0$$

解：                                            $$\frac{dy}{dx}=\frac{x-y-1}{x +4y-1}$$

$$
\begin{cases}
x-y-1=0 \\ x+4y-1=0 \\
\end{cases} \\ 解得(1,0) \\ 令 \quad x-1=X\\y=Y \\ \frac{dY}{dX}=\frac{X-Y}{X+4Y}=-\frac{1-\frac{Y}{X}}{1+4\frac{Y}{X}} \\ \frac{Y}{X}=u \\u+X\frac{du}{dX}=-\frac{1-u}{1+4u} \\ X\frac{du}{dX}=\frac{u-1-u-4u^2}{1+4u}\\-\int\frac{1+4u}{1+4u^2}=\int\frac{dX}{X}\\ \int\frac{1}{2}\frac{d(2u)}{1+4u^2}+\int\frac{1}{2}\frac{d(1+4u^2)}{1+4u^2}=-\int\frac{dX}{X}\\ \arctan{2u}+\ln{(1+4u^2)}=-2\ln{|X|}+c \\ ln(1+4(\frac{y}{x-1})^2(x-1)^2)+\arctan{\frac{2y}{x-1}}=c
$$

