# 常数变易法

形如$$\frac{dy}{dx}=P(x)y+Q(x)\tag{1}$$

$$\psi(x) \equiv 0 \quad \frac{dy}{dx}=P(x)y \tag{2}$$​

### 常数变易法

（2）的解为$$y=ce^{\int p(x)dx}$$​

设$$\hat{y}=c(x)e^{\int p(x)dx}$$（1）的一个解

$$c'(x)e^{\int p(x)dx}+c(x)p(x)e^{\int p(x)dx}=p(x)c(x)e^{\int p(x)dx}+Q(x)$$

&#x20;                                                $$c'(x)=Q(x)e^{-\int p(x)dx}$$

&#x20;                                     $$\therefore \qquad c(x)=\int Q(x)e^{-\int p(x)dx}dx$$

$$y=e^{\int p(x)dx}(\int Q(x)e^{-\int p(x)dx}dx+C)$$

​$$\quad =Ce^{\int p(x)dx} +e^{\int p(x)dx}\int Q(x)e^{-\int p(x)dx}dx$$​

&#x20;      &#x20;
